[Formal] Polymorphic (key + value) maps with typeclass
Extend total/partial maps to be polymorphic over the key in addition to
the value. This is achieved by defining a typeclass for `eqb` to be
shared by nat and string.

Test plan:

`make` to see that everything typechecks.

ghstack-source-id: 7898d9217e8549e63112a48c94cc0a1b7b3949e4
Pull Request resolved: https://github.com/JHU-PL-Lab/dde/pull/47

formal/Core.v
@@ -43,7 +43,7 @@ Notation "v @@ l" :=
 (* TODO: meh syntax to make parser happy *)
 Notation "#[ v , l , s ]" :=
   (Res v l s)
-    (in custom lang at level 15, v at level 25, s at level 25, no associativity) : lang_scope.
+    (in custom lang at level 15, v at level 25, l at level 25, s at level 25, no associativity) : lang_scope.
 
 Open Scope lang_scope.
 
@@ -62,33 +62,36 @@ Example sample_res := <{ #[ fun X -> X@0, 1, [] ] }>.
 
 (* TODO: auto-generate labels *)
 
+Definition myfun : Type := partial_map nat nat.
+Definition mylexpr : Type := partial_map nat lexpr.
+
 (* build mapping from label to label of enclosing function given a root lexpr *)
-Fixpoint build_myfun (le : lexpr) (myfun_l : option nat) (myfun : partial_map nat) : partial_map nat :=
+Fixpoint build_myfun (le : lexpr) (mf_l : option nat) (mf : myfun) : myfun :=
   match le with
   | <{ e @ l }> =>
     match e with
     | Val v =>
       match v with
-      | <{ fun _ -> e' }> => build_myfun e' (Some l) (l !-> myfun_l; myfun)
+      | <{ fun _ -> e' }> => build_myfun e' (Some l) (l !-> mf_l; mf)
       end
-    | Ident _ => (l !-> myfun_l; myfun)
-    | <{ e1 <- e2 }> => build_myfun e2 myfun_l (build_myfun e1 myfun_l myfun)
+    | Ident _ => (l !-> mf_l; mf)
+    | <{ e1 <- e2 }> => build_myfun e2 mf_l (build_myfun e1 mf_l mf)
     end
   end.
 
 (* Compute build_myfun <{ (fun X -> X@1 ) @@ 2 }> None empty. *)
 
 (* build mapping from label to lexpr given a root lexpr *)
-Fixpoint build_mylexpr (le : lexpr) (mylexpr : partial_map lexpr) : partial_map lexpr :=
+Fixpoint build_mylexpr (le : lexpr) (ml : mylexpr) : mylexpr :=
   match le with
   | <{ e @ l }> =>
     match e with
     | Val v =>
       match v with
-      | <{ fun _ -> e' }> => (l |-> le; build_mylexpr e' mylexpr)
+      | <{ fun _ -> e' }> => (l |-> le; build_mylexpr e' ml)
       end
-    | Ident _ => (l |-> le; mylexpr)
-    | <{ e1 <- e2 }> => (l |-> le; build_mylexpr e2 (build_mylexpr e1 mylexpr))
+    | Ident _ => (l |-> le; ml)
+    | <{ e1 <- e2 }> => (l |-> le; build_mylexpr e2 (build_mylexpr e1 ml))
     end
   end.
 
@@ -96,60 +99,60 @@ Fixpoint build_mylexpr (le : lexpr) (mylexpr : partial_map lexpr) : partial_map 
 
 (* custom syntax for evaluation; I try to mirror the written syntax as much as possible *)
 Reserved Notation
-         "{{ myfun , mylexpr , s }} |- e => r"
+         "{{ mf , ml , s }} |- e => r"
          (at level 40, e custom lang at level 99,
-          myfun constr, mylexpr constr, s constr, r custom lang at level 99).
+          mf constr, ml constr, s constr, r custom lang at level 99).
 
 (* logic for DDE's concrete lambda calculus operational semantics *)
-Inductive eval : lexpr -> sigma -> res -> partial_map nat -> partial_map lexpr -> Prop :=
-  | E_Val : forall s v l myfun mylexpr,
-    {{ myfun, mylexpr, s }} |- v@@l => #[ v, l, s ]
+Inductive eval : lexpr -> sigma -> res -> myfun -> mylexpr -> Prop :=
+  | E_Val : forall s v l mf ml,
+    {{ mf, ml, s }} |- v@@l => #[ v, l, s ]
   (* TODO: forall sound? *)
-  | E_Appl : forall e1 e2 l s r x e l1 s1 myfun mylexpr,
-    {{ myfun, mylexpr, s }} |- e1 => #[ fun x -> e, l1, s1 ] ->
-    {{ myfun, mylexpr, l :: s }} |- e => r ->
-    {{ myfun, mylexpr, s }} |- (e1 <- e2) @ l => r
-  | E_VarLocal : forall (x : string) l s r myfun mylexpr e1 e2 l' e myfun_l,
-    length s <> 0 ->
+  | E_Appl : forall e1 e2 l s r x e l1 s1 mf ml,
+    {{ mf, ml, s }} |- e1 => #[ fun x -> e, l1, s1 ] ->
+    {{ mf, ml, l :: s }} |- e => r ->
+    {{ mf, ml, s }} |- (e1 <- e2) @ l => r
+  | E_VarLocal : forall (x : string) l s r mf ml e1 e2 l' e mf_l,
+    List.length s <> 0 ->
     (* hd will never give default *)
-    mylexpr (hd 0 s) = Some <{ (e1 <- e2) @ l' }> ->
-    myfun l = Some myfun_l ->
-    mylexpr myfun_l = Some <{ (fun x -> e) @@ myfun_l }> ->
-    {{ myfun, mylexpr, tl s }} |- e2 => r ->
-    {{ myfun, mylexpr, s }} |- x@l => r
-  | E_VarNonLocal : forall (x : string) l s r myfun mylexpr e1 e2 l2 e myfun_l x1 s1,
-    length s <> 0 ->
-    mylexpr (hd 0 s) = Some <{ (e1 <- e2) @ l2 }> ->
-    myfun l = Some myfun_l ->
-    mylexpr myfun_l = Some <{ (fun x1 -> e) @@ myfun_l }> ->
+    ml (hd 0 s) = Some <{ (e1 <- e2) @ l' }> ->
+    mf l = Some mf_l ->
+    ml mf_l = Some <{ (fun x -> e) @@ mf_l }> ->
+    {{ mf, ml, tl s }} |- e2 => r ->
+    {{ mf, ml, s }} |- x@l => r
+  | E_VarNonLocal : forall (x : string) l s r mf ml e1 e2 l2 e mf_l x1 s1,
+    List.length s <> 0 ->
+    ml (hd 0 s) = Some <{ (e1 <- e2) @ l2 }> ->
+    mf l = Some mf_l ->
+    ml mf_l = Some <{ (fun x1 -> e) @@ mf_l }> ->
     x <> x1 ->
-    {{ myfun, mylexpr, tl s }} |- e1 => #[ fun x1 -> e, myfun_l, s1 ] ->
-    {{ myfun, mylexpr, s1 }} |- x@myfun_l => r ->
-    {{ myfun, mylexpr, s }} |- x@l => r
+    {{ mf, ml, tl s }} |- e1 => #[ fun x1 -> e, mf_l, s1 ] ->
+    {{ mf, ml, s1 }} |- x@mf_l => r ->
+    {{ mf, ml, s }} |- x@l => r
 
-  where "{{ myfun , mylexpr , s }} |- e => r" := (eval e s r myfun mylexpr).
+  where "{{ mf , ml , s }} |- e => r" := (eval e s r mf ml).
 
 Hint Unfold build_myfun build_mylexpr update t_update : core.
 
 Definition id_val :=
   <{ (fun X -> X@0) @@ 1 }>.
-Definition id_val_myfun :=
+Definition id_val_mf :=
   build_myfun id_val None empty.
-Definition id_val_mylexpr :=
+Definition id_val_ml :=
   build_mylexpr id_val empty.
 
 (* simple value *)
-Example val_correct :
-  {{ id_val_myfun, id_val_mylexpr, [] }} |- id_val => #[ fun X -> X@0, 1, [] ].
+Example eg_val_correct :
+  {{ id_val_mf, id_val_ml, [] }} |- id_val => #[ fun X -> X@0, 1, [] ].
 Proof.
   apply E_Val.
 Qed.
 
 Definition eg_loc :=
   <{ ((fun X -> X@0) @@ 1 <- (fun Y -> Y@2) @@ 3) @ 4 }>.
-Definition eg_loc_myfun :=
+Definition eg_loc_mf :=
   build_myfun eg_loc None empty.
-Definition eg_loc_mylexpr :=
+Definition eg_loc_ml :=
   build_mylexpr eg_loc empty.
 
 (* local variable lookup *)
@@ -157,15 +160,15 @@ Definition eg_loc_mylexpr :=
    so that the proof can be better traced to see what's happening. Proof
    scripts can be almost entirely automated in our logic. *)
 Example eg_loc_correct :
-  {{ eg_loc_myfun, eg_loc_mylexpr, [] }} |- eg_loc => #[ fun Y -> Y@2, 3, [] ].
+  {{ eg_loc_mf, eg_loc_ml, [] }} |- eg_loc => #[ fun Y -> Y@2, 3, [] ].
 Proof.
   eapply E_Appl.
   - apply E_Val.
   - eapply E_VarLocal.
     + auto.
-    + unfold eg_loc_mylexpr, eg_loc. autounfold. reflexivity.
-    + unfold eg_loc_myfun, eg_loc. autounfold. reflexivity.
-    + unfold eg_loc_mylexpr, eg_loc. autounfold. reflexivity.
+    + unfold eg_loc_ml, eg_loc. autounfold. reflexivity.
+    + unfold eg_loc_mf, eg_loc. autounfold. reflexivity.
+    + unfold eg_loc_ml, eg_loc. autounfold. reflexivity.
     + apply E_Val.
 Qed.
 
@@ -173,14 +176,14 @@ Definition eg_noloc :=
   <{ (((fun X -> (fun Y -> X@0) @@ 1) @@ 2
       <- (fun Z -> Z@3) @@ 4) @ 5
       <- (fun M -> M@6) @@ 7) @ 8 }>.
-Definition eg_noloc_myfun :=
+Definition eg_noloc_mf :=
   build_myfun eg_noloc None empty.
-Definition eg_noloc_mylexpr :=
+Definition eg_noloc_ml :=
   build_mylexpr eg_noloc empty.
 
 (* non-local variable lookup *)
 Example eg_noloc_correct :
-  {{ eg_noloc_myfun, eg_noloc_mylexpr, [] }} |- eg_noloc => #[ fun Z -> Z@3, 4, [] ].
+  {{ eg_noloc_mf, eg_noloc_ml, [] }} |- eg_noloc => #[ fun Z -> Z@3, 4, [] ].
 Proof.
   eapply E_Appl.
   - eapply E_Appl.
@@ -190,7 +193,7 @@ Proof.
     + auto.
     + reflexivity.
     + reflexivity.
-    + unfold eg_noloc_mylexpr, eg_noloc. autounfold. reflexivity.
+    + unfold eg_noloc_ml, eg_noloc. autounfold. reflexivity.
     + intro contra. discriminate contra.
     (* N.B. that we re-do the application here, as expected from the rules *)
     + eapply E_Appl.
@@ -213,7 +216,7 @@ Ltac map_lookup mymap prog :=
 
 (* bad non-local variable lookup *)
 Example eg_noloc_bad :
-  ~ {{ eg_noloc_myfun, eg_noloc_mylexpr, [] }} |- eg_noloc => #[ fun M -> M@6, 7, [] ].
+  ~ {{ eg_noloc_mf, eg_noloc_ml, [] }} |- eg_noloc => #[ fun M -> M@6, 7, [] ].
 Proof.
   intro contra.
   inversion contra. subst. clear contra.
@@ -222,26 +225,26 @@ Proof.
   inversion H9. subst. clear H9.
   inversion H7; subst; clear H7.
   (* E_VarLocal *)
-  - map_lookup eg_noloc_myfun eg_noloc.
-    map_lookup eg_noloc_mylexpr eg_noloc.
+  - map_lookup eg_noloc_mf eg_noloc.
+    map_lookup eg_noloc_ml eg_noloc.
     discriminate H4.
   (* E_VarNonLocal *)
-  - map_lookup eg_noloc_mylexpr eg_noloc.
-    map_lookup eg_noloc_myfun eg_noloc.
-    map_lookup eg_noloc_mylexpr eg_noloc.
+  - map_lookup eg_noloc_ml eg_noloc.
+    map_lookup eg_noloc_mf eg_noloc.
+    map_lookup eg_noloc_ml eg_noloc.
     inversion H6. subst. clear H6.
     inversion H9. subst. clear H9.
     inversion H10. subst. clear H10.
     inversion H12; subst; clear H12.
     (* E_VarLocal *)
-    + map_lookup eg_noloc_mylexpr eg_noloc.
-      map_lookup eg_noloc_myfun eg_noloc.
-      map_lookup eg_noloc_mylexpr eg_noloc.
+    + map_lookup eg_noloc_ml eg_noloc.
+      map_lookup eg_noloc_mf eg_noloc.
+      map_lookup eg_noloc_ml eg_noloc.
       inversion H11.
     (* E_VarNonLocal *)
-    + map_lookup eg_noloc_mylexpr eg_noloc.
-      map_lookup eg_noloc_myfun eg_noloc.
-      map_lookup eg_noloc_mylexpr eg_noloc.
+    + map_lookup eg_noloc_ml eg_noloc.
+      map_lookup eg_noloc_mf eg_noloc.
+      map_lookup eg_noloc_ml eg_noloc.
       contradiction.
 Qed.
 
@@ -252,9 +255,9 @@ Ltac injection_subst :=
     |- _ => rewrite H1 in H2; injection H2 as H2; subst; clear H1
   end.
 
-Theorem eval_deterministic : forall myfun mylexpr s e r1 r2,
-  {{ myfun, mylexpr, s }} |- e => r1 ->
-  {{ myfun, mylexpr, s }} |- e => r2 ->
+Theorem eval_deterministic : forall mf ml s e r1 r2,
+  {{ mf, ml, s }} |- e => r1 ->
+  {{ mf, ml, s }} |- e => r2 ->
   r1 = r2.
 Proof.
   intros. generalize dependent r2. induction H; intros.
